\documentclass[10pt, a4paper]{article}
\usepackage[T1]{fontenc}
\usepackage[left=2cm, right=2cm, top=2cm, bottom=2cm]{geometry}
\usepackage{graphicx}
\usepackage{mathtools}
\DeclareMathOperator{\arcsinh}{arcsinh}
\usepackage{amssymb}
\usepackage{wasysym} % for \astrosun and more!
\usepackage{mathrsfs} % to use \mathscr{...}
\usepackage{xcolor} % \textcolor{red}{...} & \mathcolor{red}{...}
\usepackage{hyperref} %Automatically links \label and \ref commands; Always load last
\hypersetup{
	linktocpage,
	colorlinks=true, % false: boxed links; true: colored links
	linkcolor=red, % color of internal links
	citecolor=blue, % color of links to bibliography
	filecolor=magenta, % color of file links
	urlcolor=purple, % color of external links
} % hidelinks
%----------------------------------------------------------------------
\usepackage{fancyhdr}

\pagestyle{fancy}
\fancyhf{}  % Clear all headers and footers

% Redefine section mark to include section number and title
\renewcommand{\sectionmark}[1]{%
	\markboth{Section \thesection\ #1}{}%
}

\fancyhead[L]{\nouppercase{\leftmark}}  % Header always on the left
\fancyfoot[C]{\thepage}                 % Centered page number
%----------------------------------------------------------------------
% for XeTeX
\usepackage{xeCJK}
\setCJKmainfont{GenRyuMin JP} % 源流明体
\setCJKmonofont{GenRyuMin JP} % font used in \texttt{} (just to prevent a warning)
% for LuaTeX
%\usepackage{luatexja-fontspec}
%\setmainjfont{GenRyuMin2 JP} % 源流明体
%----------------------------------------------------------------------
% to handle a large project
\usepackage{import}
%----------------------------------------------------------------------
\usepackage{indentfirst}
\setlength{\parindent}{0em} % 首行缩进
%----------------------------------------------------------------------
% horizontal line
%\noindent\rule[0.5ex]{\linewidth}{0.5pt} % horizontal line
\usepackage{dashrule}
%\noindent\hdashrule[0.5ex]{\linewidth}{0.5pt}{1mm} % horizontal dashed line
%----------------------------------------------------------------------
\usepackage[breakable]{tcolorbox} % box with color; highlight text \colorbox{yellow}{...}
\tcbset{breakable, colback=white, colframe=green!30!black, coltext=black!60!white, fonttitle=\bfseries}

\usepackage{tabularx} % LaTeX table
\usepackage{booktabs}

\usepackage{float} % appropriate way to handle figures
% example:
%\begin{figure}[H]
%	\centering
%	\includegraphics[scale=1]{figures/file-name}
%	\caption{...}
%\end{figure}
\usepackage{subcaption}
% following David Tong's convention, one should always add a caption to figures, but not to tables.
% use \vcenter{\hbox{\includegraphics[...]{...}}} to insert figures (e.g. Feynman diagrams) in equation environment.
%----------------------------------------------------------------------
\numberwithin{equation}{section}
\allowdisplaybreaks % allow page breaks inside math environments globally

\usepackage{braket}
\usepackage{cancel}

\usepackage{leftindex}
\usepackage{tensor} % how to handle indeces: https://tex.stackexchange.com/questions/11542/left-and-right-subscript-superscript
\usepackage{isotope} % e.g. \isotoe[4][2]{He} = helium-4

\usepackage{simpler-wick} % to use Wick contraction
%\usepackage[compat=1.1.0]{tikz-feynman}

% use \, in math environment
% except for texts embeded in math environment, use \ instead
%----------------------------------------------------------------------
\usepackage{listings}
\lstset{
	frame=single,
	basicstyle=\ttfamily,
	numbers=left,
	numberstyle=\ttfamily,
}
%----------------------------------------------------------------------
\usepackage{orcidlink}
%----------------------------------------------------------------------
\title{\Huge \textbf{Numerical Path Integral}}
\author{Siyang Wan (万思扬)}
\date{June 2, 2025}
%----------------------------------------------------------------------
\begin{document}
	\maketitle
	
	\pdfbookmark[1]{\contentsname}{toc} % add pdf bookmark to the ToC
	\tableofcontents
	
	\section{path integral in quantum mechanics}
	\begin{itemize}
		\item 考虑系统的 Hamiltonian 为
		\begin{equation}
			H = \frac{p^2}{2 m} + V(x),
		\end{equation}
		那么其 Lagrangian 为
		\begin{equation}
			L = \frac{m}{2} \dot{x}^2 - V(x),
		\end{equation}
		系统初态为 $\ket{\psi_0}$.
		
		\item 用 path integral 计算 $\psi(T, x) = \braket{x | e^{- i H T} | \psi_0}$, 有
		\begin{align}
			\braket{x | e^{- i H T} | \psi_0} =& \int Dx \, e^{i \int_0^T dt \, L} \notag \\
			=& \lim_{N \rightarrow \infty} \int dx_0 \, \psi_0(x_0) \int dx_{N + 1} \, \delta(x_{N + 1} - x) \notag \\
			& \int dx_1 \cdots dx_N \, \exp \Big( i \sum_{i = 0}^N \Delta t \Big( \frac{m}{2} \Big( \frac{x_{i + 1} - x_i}{\Delta t} \Big)^2 - V(x_i) \Big) \Big),
		\end{align}
		其中 $\Delta t = \frac{T}{N + 1}$.
		
		\item 数值计算中, 令
		\begin{equation}
			\begin{dcases}
				x_i = \Big( \frac{2 i}{M} - 1 \Big) L, \Delta x = \frac{2 L}{M}, i = 0, \cdots, M \\
				K_{i j} = \braket{x_i | e^{- i H \Delta t} | x_j} = \sqrt{\frac{m}{2 \pi i \Delta t}} \exp \Big( i \Big( \frac{m}{2} \frac{(x_i - x_j)^2}{\Delta t} - \Delta t V(x_i) \Big) \Big)
			\end{dcases},
		\end{equation}
		那么
		\begin{equation} \label{1.5}
			\braket{x | e^{- i H T} | \psi_0} = \lim_{L, M, N \rightarrow \infty} (\Delta x)^{N + 1} \sum_{j = 0}^M (K^{N + 1})_{i j} \psi_0(x_j), \quad \text{with} \quad x_i = x \ll L.
		\end{equation}
	\end{itemize}
	
	\subsection{Gaussian wave packet}
	\begin{itemize}
		\item 考虑一个自由粒子, 初态为
		\begin{equation}
			\psi_0(x) = \Big( \frac{2}{\pi} \Big)^{\frac{1}{4}} e^{- x^2 + i k_0 x}, \quad \braket{k | \psi_0} = \frac{1}{(2 \pi)^{1 / 4}} e^{- \frac{1}{4} (k - k_0)^2},
		\end{equation}
		那么, 预期结果为
		\begin{equation}
			\psi(t, x) = \Big( \frac{2}{\pi} \Big)^{\frac{1}{4}} \sqrt{\frac{m}{m + 2 i t}} \exp \Big( \frac{m}{m + 2 i t} (- x^2 + i k_0 x) - i \frac{k_0^2}{2 (m + 2 i t)} t \Big).
		\end{equation}
		
		\item 计算 \eqref{1.5} 最快 (且节省内存) 的方法是 (每一步计算都得到向量, 而不是矩阵):
		\begin{lstlisting}
psi_final = psi_0
for i in range(N+1):
	psi_final = dx * K @ psi_final
		\end{lstlisting}
		不推荐以下两种方法 (在 $T = 0.1, L = 300, M = 9000, N = 1$ 时可以得到较准确的波形):
		\begin{lstlisting}
K_power = K
for i in range(N):
	K_power = K @ K_power
psi_final = dx**(N + 1) * K_power @ psi_0
		\end{lstlisting}
		或
		\begin{lstlisting}
K_power = np.linalg.matrix_power(K, N + 1)
psi_final = dx**(N + 1) * K_power @ psi_0
		\end{lstlisting}
		
		\item 另外, 根据经验, 需要有 $\big| \Delta x \sqrt{\frac{m}{2 \pi i \Delta t}} \big|^2 \ll 1$, 可以选取 $\sim 10^{- 2}$.
		
		\item 令 $m = k_0 = 1$, 数值计算得到的结果如下图所示 (其中 $A = \int dx \, \rho$ 是数值计算得到的 normalization constant):
		
		\begin{figure}[H]
			\centering
			\includegraphics[scale=0.8]{figures/numerical path integral (normalized) of a free particle with initial state as a Gaussian wave packet and T=1 (L=400, M=24000, N=10).pdf}
			\caption{numerical path integral (normalized) at $T = 1$ with $A \sim 10^{18}, \Delta \phi \approx \pi + 0.7$.}
		\end{figure}
	\end{itemize}
	
	\subsection{harmonic oscillator and coherent states}
	\begin{itemize}
		\item 考虑谐振子的 coherent states,
		\begin{equation}
			\begin{dcases}
				\psi^{(\alpha)}(t, x) = \Big( \frac{m \omega}{\pi} \Big)^{\frac{1}{4}} \exp \Big( - \frac{m \omega}{2} (x - \braket{x})^2 + i \braket{p} x + i \theta(t) \Big) \\
				\braket{x} = \sqrt{\frac{2}{m \omega}} \mathrm{Re}(\alpha e^{- i \omega t}), \braket{p} = \sqrt{2 m \omega} \mathrm{Im}(\alpha e^{- i \omega t}) \\
				\theta(t) = - \frac{\omega t}{2} - \mathrm{Re}(\alpha e^{- i \omega t}) \mathrm{Im}(\alpha e^{- i \omega t})
			\end{dcases},
		\end{equation}
		其中 $\alpha \in \mathbb{C}$.
		
		\item 令 $m = \omega = 1$, 考虑初始条件为 $\alpha = |\alpha| = 1$ 的情况. 计算中可以让
		\begin{equation}
			K_{i j} = \sqrt{\frac{m}{2 \pi i \Delta t}} \exp \Big( i \frac{m}{2} \frac{(x_i - x_j)^2}{\Delta t} \Big) \frac{e^{- i \Delta t V(x_i)} + e^{- i \Delta t V(x_j)}}{2},
		\end{equation}
		这对数值结果有微小的改进.
		
		\item 数值计算结果如下:
		
		\begin{figure}[H]
			\centering
			\includegraphics[scale=0.8]{figures/numerical path integral (normalized) of a harmonic oscillator with initial state as a coherent state and T=frac{pi}{2} (L=30, M=16000, N=15).pdf}
			\caption{numerical path integral at $T = \frac{\pi}{2}$.}
		\end{figure}
		
		注意到, coherent state 用路径积分数值计算得到的结果具有正确的归一化系数 $A = 1$ 和相位.
	\end{itemize}
	
	\appendix
	\renewcommand{\sectionmark}[1]{%
		\markboth{Appendix \thesection\ #1}{}%
	}
	\section{coherent states}
	\begin{itemize}
		\item 参考: \href{https://en.wikipedia.org/wiki/Coherent_state}{Wikipedia: Coherent state}, \href{https://en.wikipedia.org/wiki/Displacement_operator}{Wikipedia: Displacement operator}.
		
		\item coherent states, $\ket{\alpha}$, 是 annihilation operator 的本征态
		\begin{equation}
			\begin{dcases}
				a \ket{\alpha} = \alpha \ket{\alpha}, \alpha \in \mathbb{C} \\
				\ket{\alpha} = D(\alpha) \ket{0}
			\end{dcases},
		\end{equation}
		其中 $D(\alpha)$ 是 displacement operator,
		\begin{equation}
			D(\alpha) := e^{\alpha a^\dag - \alpha^* a}.
		\end{equation}
		
		\begin{tcolorbox}[title=calculation:]
			\begin{align}
				& \begin{dcases}
					[a, (\alpha a^\dag - \alpha^* a)^n] = n \alpha (\alpha a^\dag - \alpha^* a)^{n - 1} \\
					[a^\dag, (\alpha a^\dag - \alpha^* a)^n] = n \alpha^* (\alpha a^\dag - \alpha^* a)^{n - 1} \\
					[a^\dag a, (\alpha a^\dag - \alpha^* a)^n] = n (\alpha a^\dag + \alpha^* a) (\alpha a^\dag - \alpha^* a)^{n - 1} - n (n - 1) |\alpha|^2 (\alpha a^\dag - \alpha^* a)^{n - 2}
				\end{dcases} \notag \\
				\Longrightarrow & \begin{dcases}
					[a, e^{\alpha a^\dag - \alpha^* a}] = \alpha e^{\alpha a^\dag - \alpha^* a} \\
					[a^\dag, e^{\alpha a^\dag - \alpha^* a}] = \alpha^* e^{\alpha a^\dag - \alpha^* a} \\
					[a^\dag a, e^{\alpha a^\dag - \alpha^* a}] = (\alpha a^\dag + \alpha^* a - |\alpha|^2) e^{\alpha a^\dag - \alpha^* a}
				\end{dcases},
			\end{align}
			因此
			\begin{equation} \label{A.4}
				\begin{dcases}
					a \ket{\alpha} = \cdots \\
					a^\dag \ket{\alpha} = e^{\alpha a^\dag - \alpha^* a} \ket{1} + \alpha^* \ket{\alpha} \\
					a^\dag a \ket{\alpha} = \alpha a^\dag \ket{\alpha} \Longrightarrow \braket{\alpha | a^\dag a | \alpha} = |\alpha|^2 \braket{\alpha | \alpha}
				\end{dcases}.
			\end{equation}
		\end{tcolorbox}
		
		\item displacement operator 是 unitary operator, 且满足
		\begin{equation}
			\begin{dcases}
				D(\alpha) := e^{\alpha a^\dag - \alpha^* a} = e^{- \frac{1}{2} |\alpha|^2} e^{\alpha a^\dag} e^{- \alpha^* a} = e^{\frac{1}{2} |\alpha|^2} e^{- \alpha^* a} e^{\alpha a^\dag} \\
				D(\alpha) D(\beta) = e^{\frac{1}{2} (\alpha \beta^* - \alpha^* \beta)} D(\alpha + \beta) \\
				D^\dag(\alpha) = D(- \alpha) \\
				D^\dag(\alpha) a D(\alpha) = a + \alpha \\
				D^\dag(\alpha) a^\dag D(\alpha) = a ^\dag + \alpha^*
			\end{dcases}.
		\end{equation}
		
		\begin{tcolorbox}[title=calculation:]
			首先
			\begin{equation}
				D^\dag(\alpha) = \sum_{n = 0}^\infty \frac{1}{n!} ((\alpha a^\dag - \alpha^* a)^\dag)^n = \sum_{n = 0}^\infty \frac{1}{n!} (\alpha^* a - \alpha a^\dag)^n = D(- \alpha),
			\end{equation}
			使用 BCH formula,
			\begin{align}
				& \begin{dcases}
					e^A e^B = \exp \Big( A + B + \frac{1}{2} [A, B] + \frac{1}{12} [A, [A, B]] - \frac{1}{12} [B, [A, B]] + \cdots \Big) \\
					e^A B e^{- A} = e^{\mathrm{ad}_A} B
				\end{dcases} \notag \\
				\Longrightarrow & \begin{dcases}
					e^{\alpha a^\dag} e^{- \alpha^* a} = e^{\alpha a^\dag - \alpha^* a + \frac{1}{2} |\alpha|^2} \\
					D(\alpha) D(\beta) = e^{\alpha a^\dag - \alpha^* a} e^{\beta a^\dag - \beta^* a} = D(\alpha + \beta) e^{\frac{1}{2} (\alpha \beta^* - \alpha^* \beta)} \\
					D(\alpha) D(- \alpha) = 1 \\
					e^{- (\alpha a^\dag - \alpha^* a)} a e^{\alpha a^\dag - \alpha^* a} = \exp(- \mathrm{ad}_{(\alpha a^\dag - \alpha^* a)}) a = a + \alpha \\
					e^{- (\alpha a^\dag - \alpha^* a)} a^\dag e^{\alpha a^\dag - \alpha^* a} = \exp(- \mathrm{ad}_{(\alpha a^\dag - \alpha^* a)}) a^\dag = a^\dag + \alpha^*
				\end{dcases}.
			\end{align}
		\end{tcolorbox}
		
		\item coherent states 满足
		\begin{equation}
			\begin{dcases}
				\braket{\alpha | a^\dag a | \alpha} = |\alpha|^2 \braket{\alpha | \alpha} \\
				\braket{n | \alpha} = \frac{\alpha^n}{\sqrt{n!}} \braket{0 | D(\alpha) | 0} = \frac{\alpha^n}{\sqrt{n!}} e^{- \frac{1}{2} |\alpha|^2} \\
				\braket{\alpha | \beta} = \braket{0 | D(- \alpha) D(\beta) | 0} = e^{- \frac{1}{2} (|\alpha|^2 + |\beta|^2 - 2 \alpha^* \beta)}
			\end{dcases}.
		\end{equation}
		
		\begin{tcolorbox}[title=calculation:]
			注意
			\begin{equation}
				\begin{dcases}
					[a, (a^\dag)^n] = n (a^\dag)^{n - 1} \\
					\braket{0 | a^n (a^\dag)^n | 0} = n!
				\end{dcases} \Longrightarrow \ket{n} = \frac{(a^\dag)^n}{\sqrt{n!}} \ket{0},
			\end{equation}
			那么
			\begin{equation}
				\braket{n | \alpha} = \braket{n | e^{\alpha a^\dag - \alpha^* a} | 0} = \frac{1}{\sqrt{n!}} \sum_{m = 0}^\infty \frac{1}{m!} \braket{0 | a^n (\alpha a^\dag - \alpha^* a)^m | 0},
			\end{equation}
			其中
			\begin{align}
				\braket{0 | a^n (\alpha a^\dag - \alpha^* a)^m | 0} &= m \alpha \braket{0 | a^{n - 1} (\alpha a^\dag - \alpha^* a)^{m - 1} | 0} \notag \\
				&= \begin{dcases}
					0 & m < n \\
					\frac{m! \alpha^n}{(m - n)!} \braket{0 | (\alpha a^\dag - \alpha^* a)^{m - n} | 0} & m \geq n
				\end{dcases},
			\end{align}
			代入, 得
			\begin{equation}
				\braket{n | \alpha} = \frac{\alpha^n}{\sqrt{n!}} \braket{0 | D(\alpha) | 0},
			\end{equation}
			其中
			\begin{align}
				\braket{0 | D(\alpha) | 0} = \braket{0 | e^{- \frac{1}{2} |\alpha|^2} e^{\alpha a^\dag} e^{- \alpha^* a} | 0} = e^{- \frac{1}{2} |\alpha|^2}.
			\end{align}
		\end{tcolorbox}
		
		\item 因此
		\begin{equation}
			I = \frac{1}{\pi} \int d^2 \alpha \, \ket{\alpha} \bra{\alpha}, \quad d^2 \alpha \equiv d\mathrm{Re}(\alpha) d\mathrm{Im}(\alpha).
		\end{equation}
		
		\begin{tcolorbox}[title=proof:]
			考虑
			\begin{align}
				\int d^2 \alpha \, \braket{m | \alpha} \braket{\alpha | n} &= \frac{1}{\sqrt{m! n!}} \int d^2 \alpha \, \alpha^m (\alpha^*)^n e^{- |\alpha|^2} \notag \\
				&= \frac{1}{\sqrt{m! n!}} \int_0^\infty r dr \int_0^{2 \pi} d\theta \, r^{m + n} e^{i (m - n) \theta} e^{- r^2} \notag \\
				&= \begin{dcases}
					0 & m \neq n \\
					\frac{2 \pi}{n!} \int_0^\infty dr \, r^{2 n + 1} e^{- r^2} & m = n
				\end{dcases} = \pi \delta_{m n}.
			\end{align}
		\end{tcolorbox}
		
		\item $a^\dag$ 没有 eigenket, 但有
		\begin{equation}
			a^\dag \ket{\alpha} \bra{\alpha} = \Big( \frac{\partial}{\partial \alpha} + \alpha^* \Big) \ket{\alpha} \bra{\alpha}.
		\end{equation}
		
		\begin{tcolorbox}[title=proof:]
			根据 \eqref{A.4}, 有
			\begin{equation}
				a^\dag \ket{\alpha} \bra{\alpha} = e^{\alpha a^\dag - \alpha^* a} \ket{1} \bra{\alpha} + \alpha^* \ket{\alpha} \bra{\alpha},
			\end{equation}
			并且
			\begin{align}
				\frac{\partial}{\partial \alpha} \ket{\alpha} \bra{\alpha} &= \frac{\partial}{\partial \alpha} \Big( e^{\frac{1}{2} |\alpha|^2} e^{- \alpha^* a} e^{\alpha a^\dag} \ket{0} \bra{0} e^{- \frac{1}{2} |\alpha|^2} e^{- \alpha a^\dag} e^{\alpha^* a} \Big) \notag \\
				&= D(\alpha) \Big( \frac{1}{2} \alpha^* + a^\dag \Big) \ket{0} \bra{\alpha} + \ket{\alpha} \bra{0} \Big( - \frac{1}{2} \alpha^* - a^\dag \Big) D(- \alpha) \notag \\
				&= D(\alpha) \ket{1} \bra{\alpha} - \ket{\alpha} \bra{1} D(- \alpha)
			\end{align}
		\end{tcolorbox}
	\end{itemize}
\end{document}